coqimp/framework/models/language.v
@@ -37,6 +37,7 @@ Inductive command: Type :=
 | ccall : Label -> command
 | cjumpl : AddrExp -> GenReg -> command
 | cretl : command
+| cret : command
 | cbe : Label -> command
 | cbne : Label -> command.
 
@@ -46,6 +47,7 @@ Inductive InsSeq : Type :=
 | consJ : AddrExp -> GenReg -> ins -> InsSeq
 | consCall : Label -> ins -> InsSeq -> InsSeq
 | consRetl : ins -> InsSeq
+| consRet : ins -> InsSeq
 | consBe : Label -> ins -> InsSeq -> InsSeq
 | consBne : Label -> ins -> InsSeq -> InsSeq.
 
@@ -69,6 +71,9 @@ Notation " 'call' f # i # I" :=
 Notation "'retl' ;; i" :=
   (consRetl i) (at level 80, right associativity): code_scope.
 
+Notation "'ret' ;; i" :=
+  (consRet i) (at level 80, right associativity): code_scope.
+
 Notation "'be' f # i # I" :=
   (consBe f i I) (at level 90, right associativity,
                      format
@@ -80,6 +85,33 @@ Notation "'bne' f # i # I" :=
                    format
                      "'bne' '/' f # i # '//' I"
                   ): code_scope.
+
+(* Test code *)
+Definition f1 := ($ 1).
+Definition f2 := ($ 2).
+Definition f3 := ($ 3).
+Definition f4 := ($ 4).
+
+Definition code : InsSeq := 
+  consJ (Ao (Or r1)) r3 nop. 
+Print code.
+
+Definition code1 : InsSeq :=
+  consSeq (add r1 (Or r2) r3) (consJ (Ao (Or r1)) r3 nop).
+Print code1.
+
+Definition code2 : InsSeq :=
+  retl ;; nop.
+
+Definition code3 : InsSeq :=
+  nop ;; (add r1 (Or r1) r2) ;;
+      retl ;; nop.
+
+Definition code4 : InsSeq :=
+  call f3 # nop # code3.
+
+Definition code5 : InsSeq :=
+  be f3 # nop # code3.
 
 Open Scope code_scope.
 
@@ -102,6 +134,10 @@ Inductive LookupC : CodeHeap -> Label -> InsSeq -> Prop :=
     forall C f i,
       C f = Some (cretl) -> C (f +ᵢ ($ 4)) = Some (cntrans i) ->
       LookupC C f (retl ;; i)
+| lookupRet :
+    forall C f i,
+      C f = Some (cret) -> C (f +ᵢ ($ 4)) = Some (cntrans i) ->
+      LookupC C f (ret ;; i)
 | lookupCall :
     forall C f f' i I,
       C f = Some (ccall f') -> C (f +ᵢ ($ 4)) = Some (cntrans i) ->
@@ -129,10 +165,10 @@ Definition word_aligned: Word -> bool :=
 Definition iszero v :=
   if Int.eq_dec v ($ 0) then $ 1 else $ 0.
 
-Fixpoint set_Rs (R : RegFile) (lv : list (RegName * Word)) :=
-  match lv with
-  | (rn, v) :: lv' =>
-    set_Rs (RegMap.set rn v R) lv'
+Fixpoint set_Rs R (vl : list (RegName * Word)) :=
+  match vl with
+  | (rr, w) :: vl =>
+    set_Rs (set_R R rr w) vl
   | nil => R
   end.
 
@@ -140,68 +176,85 @@ Fixpoint set_Rs (R : RegFile) (lv : list (RegName * Word)) :=
 Inductive R__ : Memory * RegFile -> ins -> Memory * RegFile -> Prop :=
 | Ld_step : forall aexp (ri : GenReg) M R R' addr v,
     eval_addrexp R aexp = Some addr -> word_aligned addr = true ->
-    M addr = Some v -> RegMap.set ri v R = R' ->
+    M addr = Some v -> indom ri R -> set_R R ri v = R' ->
     R__ (M, R) (ld aexp ri) (M, R')
 
 | ST_step : forall (ri : GenReg) aexp M M' R addr v,
     eval_addrexp R aexp = Some addr -> word_aligned addr = true ->
-    get_R R ri = v -> indom addr M -> MemMap.set addr (Some v) M = M' ->
+    get_R R ri = Some v -> indom addr M -> MemMap.set addr (Some v) M = M' ->
     R__ (M, R) (st ri aexp) (M', R)
 
 | Nop_step : forall M R,
     R__ (M, R) nop (M, R)
 
 | Add_step : forall M (R R' : RegFile) oexp (rs rd : GenReg) v1 v2,
-    get_R R rs = v1 -> eval_opexp R oexp = Some v2 ->
-    RegMap.set rd (v1 +ᵢ v2) R = R' ->
+    get_R R rs = Some v1 -> eval_opexp R oexp = Some v2 ->
+    indom rd R -> set_R R rd (v1 +ᵢ v2) = R' ->
     R__ (M, R) (add rs oexp rd) (M, R')
         
 | Sub_step : forall M (R R' : RegFile) oexp (rs rd : GenReg) v1 v2,
-    get_R R rs = v1 -> eval_opexp R oexp = Some v2 ->
-    RegMap.set rd (v1 -ᵢ v2) R = R' ->
+    get_R R rs = Some v1 -> eval_opexp R oexp = Some v2 ->
+    indom rd R -> set_R R rd (v1 -ᵢ v2) = R' ->
     R__ (M, R) (sub rs oexp rd) (M, R')
 
 | Subcc_step : forall M (R R' : RegFile) oexp (rs rd : GenReg) v1 v2 v,
-    get_R R rs = v1 -> eval_opexp R oexp = Some v2 -> v = v1 -ᵢ v2 ->
+    get_R R rs = Some v1 -> eval_opexp R oexp = Some v2 ->
+    indom rd R -> indom n R -> indom z R -> v = v1 -ᵢ v2 ->
     set_Rs R ((Rr rd, v) :: (Rpsr n, get_range 31 31 v) :: (Rpsr z, iszero v) :: nil) = R' ->
     R__ (M, R) (subcc rs oexp rd) (M, R')
 
 | And_step : forall M (R R' : RegFile) oexp (rs rd : GenReg) v1 v2,
-    get_R R rs = v1 -> eval_opexp R oexp = Some v2 ->
-    RegMap.set rd (v1 &ᵢ v2) R = R' ->
+    get_R R rs = Some v1 -> eval_opexp R oexp = Some v2 ->
+    indom rd R -> set_R R rd (v1 &ᵢ v2) = R' ->
     R__ (M, R) (and rs oexp rd) (M, R')
 
 | Andcc_step : forall M (R R' : RegFile) oexp (rs rd : GenReg) v1 v2 v,
-    get_R R rs = v1 -> eval_opexp R oexp = Some v2 -> v = v1 &ᵢ v2 ->
+    get_R R rs = Some v1 -> eval_opexp R oexp = Some v2 ->
+    indom rd R -> indom n R -> indom z R -> v = v1 &ᵢ v2 ->
     set_Rs R ((Rr rd, v) :: (Rpsr n, get_range 31 31 v) :: (Rpsr z, iszero v) :: nil) = R' ->
     R__ (M, R) (andcc rs oexp rd) (M, R')
 
 | Or_step : forall M (R R' : RegFile) oexp (rs rd : GenReg) v1 v2,
-    get_R R rs = v1 -> eval_opexp R oexp = Some v2 ->
-    RegMap.set rd (v1 |ᵢ v2) R = R' ->
+    get_R R rs = Some v1 -> eval_opexp R oexp = Some v2 ->
+    indom rd R -> set_R R rd (v1 |ᵢ v2) = R' ->
     R__ (M, R) (or rs oexp rd) (M, R')
 
 | Sll_step : forall M (R R' : RegFile) oexp (rs rd : GenReg) v1 v2,
-    get_R R rs = v1 -> eval_opexp R oexp = Some v2 ->
-    RegMap.set rd (v1 <<ᵢ (get_range 0 4 v2)) R = R' ->
+    get_R R rs = Some v1 -> eval_opexp R oexp = Some v2 ->
+    indom rd R -> set_R R rd (v1 <<ᵢ (get_range 0 4 v2)) = R' ->
     R__ (M, R) (sll rs oexp rd) (M, R')
 
 | Srl_step : forall M (R R' : RegFile) oexp (rs rd : GenReg) v1 v2,
-    get_R R rs = v1 -> eval_opexp R oexp = Some v2 ->
-    RegMap.set rd (v1 >>ᵢ (get_range 0 4 v2)) R = R' ->
+    get_R R rs = Some v1 -> eval_opexp R oexp = Some v2 ->
+    indom rd R -> set_R R rd (v1 >>ᵢ (get_range 0 4 v2)) = R' ->
     R__ (M, R) (srl rs oexp rd) (M, R')
 
 | Set_step : forall M (R R' : RegFile) (rd : GenReg) w,
-    RegMap.set rd w R = R' ->
+    indom rd R -> set_R R rd w = R' ->
     R__ (M, R) (sett w rd) (M, R')
 
 | Rd_step : forall M (R R' : RegFile) (rsp : SpReg) (ri : GenReg) v,
-    get_R R rsp = v -> RegMap.set ri v R = R' ->
+    get_R R rsp = Some v -> indom ri R -> set_R R ri v = R' ->
     R__ (M, R) (rd rsp ri) (M, R')
 
 | GetCwp_step : forall M (R R' : RegFile) (ri : GenReg) v,
-    get_R R cwp = v -> RegMap.set ri v R = R' ->
+    get_R R cwp = Some v -> indom ri R -> set_R R ri v = R' ->
     R__ (M, R) (getcwp ri) (M, R').
+
+(* Operation to write a frame *)
+Definition set_frame R (rr0 rr1 rr2 rr3 rr4 rr5 rr6 rr7 : GenReg) (fm : Frame) :=
+  match fm with
+  | consfm w0 w1 w2 w3 w4 w5 w6 w7 =>
+    set_Rs R
+           ((Rr rr0, w0) :: (Rr rr1, w1) :: (Rr rr2, w2) :: (Rr rr3, w3) :: (Rr rr4, w4) ::
+                         (Rr rr5, w5) :: (Rr rr6, w6) :: (Rr rr7, w7) :: nil)
+  end.
+
+(* Operation to write a window *)
+Definition set_window R (fm1 fm2 fm3 : Frame) :=
+  let R1 := set_frame R r8 r9 r10 r11 r12 r13 r14 r15 fm1 in
+  let R2 := set_frame R1 r16 r17 r18 r19 r20 r21 r22 r23 fm2 in
+  set_frame R2 r24 r25 r26 r27 r28 r29 r30 r31 fm3.
 
 Definition N := $ 8.
 
@@ -229,28 +282,28 @@ Inductive Q__: State -> command -> State -> Prop :=
 
 | SSave :
     forall (M : Memory) (R R' R'': RegFile) D F F' k k' oexp
-      fmo fml fmi fm1 fm2 v1 v2 v (rs rd : GenReg),
-      get_R R cwp = k -> get_R R Rwim = v ->
-      fetch R = (fmo, fml, fmi) ->
-      get_R R rs = v1 -> eval_opexp R oexp = Some v2 -> F = F' ++ (fm1 :: fm2 :: nil) ->
-      R' = replace fm1 fm2 fmo R -> k' = pre_cwp k -> win_masked k' v = false ->
+           fmo fml fmi fm1 fm2 v1 v2 v (rs rd : GenReg),
+      get_R R cwp = Some k -> get_R R Rwim = Some v ->
+      fetch R = Some [fmo; fml; fmi] -> indom rd R -> 
+      get_R R rs = Some v1 -> eval_opexp R oexp = Some v2 -> F = F' ++ (fm1 :: fm2 :: nil) ->
+      R' = set_window R fm1 fm2 fmo -> k' = pre_cwp k -> win_masked k' v = false -> 
       R'' = set_Rs R' ((Rpsr cwp, k') :: (Rr rd, v1 +ᵢ v2) :: nil) ->
       Q__ (M, (R, F), D) (cntrans (save rs oexp rd)) (M, (R'', fml :: fmi :: F'), D)
 
 | RRestore :
     forall (M : Memory) (R R' R'': RegFile) D F F' k k' oexp
-      fmo fml fmi fm1 fm2 v1 v2 v (rs rd : GenReg),
-      get_R R cwp = k -> get_R R Rwim = v ->
-      fetch R = (fmo, fml, fmi) ->
-      get_R R rs = v1 -> eval_opexp R oexp = Some v2 -> F = fm1 :: fm2 :: F' ->
-      R' = replace fmi fm1 fm2 R -> k' = post_cwp k -> win_masked k' v = false ->
+           fmo fml fmi fm1 fm2 v1 v2 v (rs rd : GenReg),
+      get_R R cwp = Some k -> get_R R Rwim = Some v ->
+      fetch R = Some [fmo; fml; fmi] -> indom rd R ->
+      get_R R rs = Some v1 -> eval_opexp R oexp = Some v2 -> F = fm1 :: fm2 :: F' ->
+      R' = set_window R fmi fm1 fm2 -> k' = post_cwp k -> win_masked k' v = false ->
       R'' = set_Rs R' ((Rpsr cwp, post_cwp k) :: (Rr rd, v1 +ᵢ v2) :: nil) ->
       Q__ (M, (R, F), D) (cntrans (restore rs oexp rd)) (M, (R'', F' ++ (fmo :: fml :: nil)), D)
-      
+
 | Wr :
     forall M (R : RegFile) F D D' (rs : GenReg) (rsp : SpReg) oexp v1 v2 v,
-      get_R R rs = v1 -> eval_opexp R oexp = Some v2 ->
-      v = set_spec_reg rsp (v1 xor v2) -> D' = set_delay rsp v D ->
+      get_R R rs = Some v1 -> eval_opexp R oexp = Some v2 ->
+      v = set_spec_reg rsp (v1 xor v2) -> indom rsp R -> D' = set_delay rsp v D ->
       Q__ (M, (R, F), D) (cntrans (wr rs oexp rsp)) (M, (R, F), D').
 
 (* Operation Semantics for Control Transfer *)
@@ -263,37 +316,42 @@ Inductive H__ : CodeHeap -> State * Label * Label -> State * Label * Label -> Pr
 | Jumpl :
     forall C M aexp rd (R R' : RegFile) F D (pc npc f : Label),
       C pc = Some (cjumpl aexp rd) -> eval_addrexp R aexp = Some f ->
-      word_aligned f = true -> RegMap.set rd pc R = R' ->
+      word_aligned f = true -> indom rd R -> set_R R rd pc = R' ->
       H__ C ((M, (R, F), D), pc, npc) ((M, (R', F), D), npc, f)
 
 | Call :
     forall C M (R R' : RegFile) F D pc npc f,
-      C pc = Some (ccall f) -> RegMap.set r15 pc R = R' ->
+      C pc = Some (ccall f) -> indom r15 R -> set_R R r15 pc = R' ->
       H__ C ((M, (R, F), D), pc, npc) ((M, (R', F), D), npc, f)
 
 | Retl :
     forall C M (R : RegFile) F D pc npc f,
-      C pc = Some (cretl) -> get_R R r15 = f ->
+      C pc = Some (cretl) -> get_R R r15 = Some f ->
+      H__ C ((M, (R, F), D), pc, npc) ((M, (R, F), D), npc, f +ᵢ ($ 8))
+
+| Ret :
+    forall C M (R : RegFile) F D pc npc f,
+      C pc = Some (cret) -> get_R R r31 = Some f ->
       H__ C ((M, (R, F), D), pc, npc) ((M, (R, F), D), npc, f +ᵢ ($ 8))
 
 | Be_true :
     forall C M (R : RegFile) F D pc npc f v,
-      C pc = Some (cbe f) -> get_R R z = v -> v <> ($ 0) ->
+      C pc = Some (cbe f) -> get_R R z = Some v -> v <> ($ 0) ->
       H__ C ((M, (R, F), D), pc, npc) ((M, (R, F), D), npc, f)
 
 | Be_false :
     forall C M (R : RegFile) F D pc npc f,
-      C pc = Some (cbe f) -> get_R R z = ($ 0) ->
+      C pc = Some (cbe f) -> get_R R z = Some ($ 0) ->
       H__ C ((M, (R, F), D), pc, npc) ((M, (R, F), D), npc, npc +ᵢ ($ 4))
 
 | Bne_true :
     forall C M (R : RegFile) F D pc npc f,
-      C pc = Some (cbne f) -> get_R R z = ($ 0) ->
+      C pc = Some (cbne f) -> get_R R z = Some ($ 0) ->
       H__ C ((M, (R, F), D), pc, npc) ((M, (R, F), D), npc, f)
 
 | Bne_false :
     forall C M (R : RegFile) F D pc npc f v,
-      C pc = Some (cbne f) -> get_R R z = v -> v <> ($ 0) ->
+      C pc = Some (cbne f) -> get_R R z = Some v -> v <> ($ 0) ->
       H__ C ((M, (R, F), D), pc, npc) ((M, (R, F), D), npc, npc +ᵢ ($ 4)).
 
 Inductive P__ : CodeHeap -> State * Label * Label -> State * Label * Label -> Prop :=
