coqimp/example/spec/spec.v
@@ -46,19 +46,34 @@ Definition add_post (vl : list logicvar) :=
   i0 |=> x ** i1 |=> y ** i2 |=> z ** l7 |=> (x +ᵢ y +ᵢ z) ** r15 |=> fret.
 
 Definition changeY_pre (vl : list logicvar) :=
-  EX fmo fml fmi fret x vy vi id fm1 fm2 F,
-  [| vl = logic_fm fmi :: logic_fm fm1 :: logic_fm fm2
-          :: logic_lv x :: logic_lv fret :: logic_lv vy :: logic_lv vi :: nil |] **
-  Regs fmo fml fmi ** Ry |=> vy ** Rwim |=> vi ** {| id, fm1 :: fm2 :: F |} **
+  EX fmg fmo fml fmi fret x vy vi id fm1 fm2 F,
+  [| vl = logic_fm fmg :: logic_fm fmi :: logic_fm fm1 :: logic_fm fm2
+          :: logic_lv x :: logic_lv fret :: logic_lv vy :: logic_lv vi :: logic_fmls F :: nil |] **
+  GenRegs (fmg, fmo, fml, fmi) ** Ry |=> vy ** Rwim |=> vi ** {| id, fm1 :: fm2 :: F |} **
   [| get_frame_nth fmi 7 = Some fret /\ get_frame_nth fmi 0 = Some x
-     /\ winvalid (post_cwp id) vi |].
+     /\ winvalid (post_cwp id) vi /\ $ 0 <=ᵤᵢ id <=ᵤᵢ $ 7 |].
 
 Definition changeY_post (vl : list logicvar) :=
-  EX fmo fml fmi fret x vy vi id fm1 fm2 F,
-  [| vl = logic_fm fmi :: logic_fm fm1 :: logic_fm fm2
-          :: logic_lv x :: logic_lv fret :: logic_lv vy :: logic_lv vi :: nil |] **
-  Regs (update_frame fmi 0 vy) fm1 fm2 ** Ry |=> vy ** Ry |=> x ** Rwim |=> vi **
+  EX fmg fmo fml fmi fret x vy vi id fm1 fm2 F,
+  [| vl = logic_fm fmg :: logic_fm fmi :: logic_fm fm1 :: logic_fm fm2
+          :: logic_lv x :: logic_lv fret :: logic_lv vy :: logic_lv vi :: logic_fmls F :: nil |] **
+  GenRegs (fmg, (update_frame fmi 0 vy), fm1, fm2) ** Ry |=> x ** Rwim |=> vi **
   {| post_cwp id, F ++ (fmo :: fml :: nil) |}.
+
+Definition sum3_pre1 (vl : list logicvar) :=
+  EX x y z fret fmg fmo fml fmi id vi F fm1 fm2,
+  [| vl = logic_lv x :: logic_lv y :: logic_lv z :: logic_lv fret :: logic_fm fmg :: nil |] **
+  GenRegs (fmg, fmo, fml, fmi) ** Rwim |=> vi ** {| id, F ++ (fm1 :: fm2 :: nil) |} ** 
+  [| get_frame_nth fmo 0 = Some x /\ get_frame_nth fmo 1 = Some y /\
+     get_frame_nth fmo 2 = Some z /\ get_frame_nth fmo 7 = Some fret /\
+     winvalid id vi /\ winvalid (pre_cwp id) vi /\ $ 0 <=ᵤᵢ id <=ᵤᵢ $ 7 |].
+
+Definition sum3_post1 (vl : list logicvar) :=
+  EX x y z fret fmg fmo fml fmi id vi F fm1 fm2,
+  [| vl = logic_lv x :: logic_lv y :: logic_lv z :: logic_lv fret :: logic_fm fmg :: nil |] **
+  GenRegs (fmg, fmo, fml, fmi) ** Rwim |=> vi ** {| id, F ++ (fm1 :: fm2 :: nil) |} **
+  [| get_frame_nth fmo 0 = Some (x +ᵢ y +ᵢ z) /\ get_frame_nth fmo 7 = Some fret /\
+     winvalid id vi /\ winvalid (pre_cwp id) vi /\ $ 0 <=ᵤᵢ id <=ᵤᵢ $ 7 |].
 
 Fixpoint convert_spec (ls : list (Address * fspec)) :
   funspec :=
